lean/TSLean/JS/AxiomAudit.lean
@@ -1,5 +1,6 @@
 import TSLean.JS.AxiomAuditMeta
 import TSLean.JS.ExecutionTheorems
+import TSLean.JS.FunctionTheorems
 import TSLean.JS.HeapTheorems
 
 #audit_proofs TSLean.JS
